abstract_machine.v
@@ -8,6 +8,8 @@ Module Type ABSTRACT_MACHINE.
   Parameter transition : configuration -> configuration -> Prop.
   Notation "c1 → c2" := (transition c1 c2) (at level 40, no associativity).
 
+  Axiom final_correct : forall v c, ~ c_final v → c.
+
 
   Reserved Notation "c1 →+ c2" (at level 40, no associativity).
 
@@ -33,3 +35,18 @@ Module Type DET_ABSTRACT_MACHINE <: ABSTRACT_MACHINE.
   Axiom next_correct  : forall c1 c2, next_conf c1 = Some c2 <-> c1 → c2.
 
 End DET_ABSTRACT_MACHINE.
+
+
+
+
+Module Type AM_SAFETY (AM : ABSTRACT_MACHINE).
+
+  Import AM.
+
+  Parameter good_conf : configuration -> Prop.
+
+  Axiom preservation : forall c1 c2, good_conf c1 -> c1 → c2 -> good_conf c2.
+  Axiom progress     : forall c, good_conf c -> 
+                           (exists v, c = c_final v) \/ (exists c', c → c').
+
+End AM_SAFETY.
